books/projects/smtlink/trusted/property/construct-uninterpreted.lisp
@@ -1,0 +1,55 @@
+;; Copyright (C) 2015, University of British Columbia
+;; Written (originally) by Yan Peng (19th October, 2021)
+;;
+;; License: A 3-clause BSD license.
+;; See the LICENSE file distributed with ACL2
+
+(in-package "SMT")
+(include-book "centaur/fty/top" :dir :system)
+(include-book "xdoc/top" :dir :system)
+(include-book "std/util/define" :dir :system)
+(include-book "std/strings/top" :dir :system)
+
+(include-book "../../utils/basics")
+
+(local (in-theory (enable symbol-symbol-alist-fix)))
+
+(local
+ (defthm crock1
+   (implies (consp (symbol-symbol-alist-fix formals))
+            (pseudo-termp (car (car (symbol-symbol-alist-fix formals))))))
+ )
+
+(define construct-formal-types ((formals symbol-symbol-alistp))
+  :returns (formal-decls pseudo-termp)
+  :measure (len (symbol-symbol-alist-fix formals))
+  (b* ((formals (symbol-symbol-alist-fix formals))
+       ((unless (consp formals)) ''t)
+       ((cons formal-hd formal-tl) formals)
+       ((cons formal formal-type) formal-hd))
+    `(if (,formal-type ,formal)
+         ,(construct-formal-types formal-tl)
+       ''nil)))
+
+(local
+ (defthm crock2
+   (pseudo-term-listp (symbol-list-fix formals))
+   :hints (("Goal" :in-theory (enable pseudo-term-listp
+                                      pseudo-termp
+                                      symbol-list-fix))))
+ )
+
+(define construct-uninterpreted ((name symbolp)
+                                 (formals symbol-listp)
+                                 (formal-types symbol-listp)
+                                 (return-type symbolp))
+  :returns (property pseudo-termp)
+  (b* ((name (symbol-fix name))
+       ((if (equal name 'quote))
+        (er hard? 'construct-uninterpreted=>construct-uninterpreted
+            "Function name should not be 'quote.~%"))
+       (formals (symbol-list-fix formals))
+       (formal-types (symbol-list-fix formal-types))
+       (return-type (symbol-fix return-type)))
+    `(implies ,(construct-formal-types (pairlis$ formals formal-types))
+              (,return-type (,name ,@formals)))))
