books/projects/smtlink/trusted/z3-py/translate-uninterpreted.lisp
@@ -1,0 +1,64 @@
+;; Copyright (C) 2015, University of British Columbia
+;; Written (originally) by Yan Peng (19th October, 2021)
+;;
+;; License: A 3-clause BSD license.
+;; See the LICENSE file distributed with ACL2
+
+(in-package "SMT")
+(include-book "centaur/fty/top" :dir :system)
+(include-book "xdoc/top" :dir :system)
+(include-book "std/util/define" :dir :system)
+(include-book "std/strings/top" :dir :system)
+
+(include-book "../../verified/hint-interface")
+(include-book "../property/construct-uninterpreted")
+(include-book "translate-declarations")
+(include-book "datatypes")
+
+(local (in-theory (enable paragraph-p word-p)))
+
+(define generate-uninterpreted-property ((name symbolp)
+                                         (hints uninterpreted-p))
+  :returns (property pseudo-termp)
+  (b* ((name (symbol-fix name))
+       (hints (uninterpreted-fix hints))
+       ((uninterpreted h) hints))
+    (construct-uninterpreted name h.formals h.formal-types h.return-type)))
+
+(define translate-uninterpreted-arguments ((types symbol-listp))
+  :returns (translated paragraph-p)
+  :measure (len types)
+  (b* ((types (symbol-list-fix types))
+       ((unless (consp types)) nil)
+       ((cons first rest) types)
+       (translated-type (translate-type first)))
+    (cons `(#\, #\Space ,translated-type)
+          (translate-uninterpreted-arguments rest))))
+
+(define translate-one-uninterpreted ((name symbolp)
+                                     (hints uninterpreted-p))
+  :returns (translated paragraph-p)
+  (b* ((name (symbol-fix name))
+       (hints (uninterpreted-fix hints))
+       ((uninterpreted h) hints)
+       (translated-formals
+        (translate-uninterpreted-arguments h.formal-types))
+       (translated-returns
+        (translate-uninterpreted-arguments (list h.return-type))))
+    `(,(translate-variable name) "= z3.Function("
+      #\' ,name #\' ,translated-formals ,translated-returns
+      ")" #\Newline)))
+
+(define translate-uninterpreted ((uninterpreted symbol-uninterpreted-alist-p))
+  :returns (mv (py-term paragraph-p)
+               (smt-property pseudo-term-listp))
+  :measure (len (symbol-uninterpreted-alist-fix uninterpreted))
+  (b* ((uninterpreted (symbol-uninterpreted-alist-fix uninterpreted))
+       ((unless (consp uninterpreted)) (mv nil nil))
+       ((cons first rest) uninterpreted)
+       ((cons name hints) first)
+       (first-decl (translate-one-uninterpreted name hints))
+       (first-property (generate-uninterpreted-property name hints))
+       ((mv rest-decl rest-property) (translate-uninterpreted rest)))
+    (mv (cons first-decl rest-decl)
+        (cons first-property rest-property))))
