books/projects/smtlink/verified/add-hypo-cp.lisp
@@ -30,6 +30,18 @@
             :in-theory (enable acl2::pseudo-term-substp))))
  )
 
+(define create-subst ((subst symbol-pseudo-term-alistp)
+                      (vars symbol-listp))
+  :returns (new-susbt symbol-pseudo-term-alistp)
+  :measure (len vars)
+  (b* ((subst (symbol-pseudo-term-alist-fix subst))
+       (vars (symbol-list-fix vars))
+       ((unless (consp vars)) subst)
+       ((cons vars-hd vars-tl) vars)
+       (item (assoc-equal vars-hd subst))
+       ((if item) (create-subst subst vars-tl)))
+    (create-subst (acons vars-hd vars-hd subst) vars-tl)))
+
 (define get-substed-hypo ((smt-hypo smt-hypo-p)
                           state)
   :returns (substed-hypo pseudo-termp)
@@ -41,8 +53,10 @@
                     "Formula returned by meta-extract ~p0 is not a pseudo-termp: ~p1~%"
                     h.thm hypo-thm)
                 ''t))
-       (hypo-thm-expanded (expand-lambda hypo-thm)))
-    (acl2::substitute-into-term hypo-thm-expanded h.subst)))
+       (hypo-thm-expanded (expand-lambda hypo-thm))
+       (subst (create-subst h.subst
+                            (acl2::simple-term-vars hypo-thm-expanded))))
+    (acl2::substitute-into-term hypo-thm-expanded subst)))
 
 (local (defthm crock (alistp (ev-smtcp-alist x a))))
 
@@ -54,6 +68,34 @@
   :hints (("Goal"
            :in-theory (e/d (get-substed-hypo) (w)))))
 
+(define remove-double-not ((term pseudo-termp))
+  :returns (new-term pseudo-termp)
+  (b* ((term (pseudo-term-fix term))
+       ((mv okp new-term)
+        (case-match term
+          (('not ('not x)) (mv t x))
+          (& (mv nil nil))))
+       ((unless okp) term))
+    new-term))
+
+(defthmd correctness-of-remove-double-not
+  (implies (and (pseudo-termp term) (alistp a))
+           (iff (ev-smtcp (remove-double-not term) a)
+                (ev-smtcp term a)))
+  :hints (("Goal"
+           :in-theory (e/d (remove-double-not) ()))))
+
+(defthm correctness-of-remove-double-not-corollary
+  (implies (and (smt-hypo-p smt-hypo) (alistp a))
+           (iff (ev-smtcp (remove-double-not
+                           `(not ,(get-substed-hypo smt-hypo state)))
+                          a)
+                (ev-smtcp `(not ,(get-substed-hypo smt-hypo state)) a)))
+  :hints (("Goal"
+           :in-theory (e/d () ())
+           :use ((:instance correctness-of-remove-double-not
+                            (term `(not ,(get-substed-hypo smt-hypo state))))))))
+
 (define add-hypo ((cl pseudo-term-listp)
                   (smt-hypo-lst smt-hypo-list-p)
                   state)
@@ -64,16 +106,18 @@
        ((unless (consp smt-hypo-lst)) cl)
        ((cons smt-hypo-hd smt-hypo-tl) smt-hypo-lst)
        (res-hd (get-substed-hypo smt-hypo-hd state)))
-    (cons `(not ,res-hd) (add-hypo cl smt-hypo-tl state))))
+    (cons (remove-double-not `(not ,res-hd))
+          (add-hypo cl smt-hypo-tl state))))
 
 (defthm correctness-of-add-hypo
   (implies (and (ev-smtcp-meta-extract-global-facts)
                 (pseudo-term-listp cl)
+                (smt-hypo-list-p hypo-lst)
                 (alistp a)
                 (ev-smtcp (disjoin (add-hypo cl hypo-lst state)) a))
            (ev-smtcp (disjoin cl) a))
   :hints (("Goal"
-           :in-theory (enable add-hypo))))
+           :in-theory (e/d (add-hypo) ()))))
 
 (define add-hypo-cp ((cl pseudo-term-listp)
                      (hints t)
@@ -82,8 +126,8 @@
        (cl (pseudo-term-list-fix cl))
        (next-cp (cdr (assoc-equal 'add-hypo *SMT-architecture*)))
        ((if (null next-cp)) (value (list cl)))
-       (the-hint `(:clause-processor (,next-cp clause ',hints state)))
-       (new-cl (add-hypo cl (smtlink-hint->hypotheses hints) state)))
+       (new-cl (add-hypo cl (smtlink-hint->hypotheses hints) state))
+       (the-hint `(:clause-processor (,next-cp clause ',hints state))))
     (value (list `((hint-please ',the-hint) ,@new-cl)))))
 
 (defthm correctness-of-add-hypos
